Completed minimal verification of exception handler

pkvm_handler/a7400.v
@@ -18,10 +18,10 @@ Definition a7400 : list trc := [
     AssumeReg "SCR_EL3" [] (RegVal_Base (Val_Bits [BV{32%N} 0x401%Z])) Mk_annot;
     AssumeReg "SCTLR_EL2" [] (RegVal_Base (Val_Bits [BV{64%N} 0x4000002%Z])) Mk_annot;
     Smt (DeclareConst 29%Z (Ty_BitVec 64%N)) Mk_annot;
-    Assume (AExp_Binop (Eq) (AExp_Manyop (Bvmanyarith Bvand) [AExp_Binop ((Bvarith Bvsub)) (AExp_Val (AVal_Var "SP_EL2" []) Mk_annot) (AExp_Val (AVal_Bits [BV{64%N} 0x8%Z]) Mk_annot) Mk_annot; AExp_Val (AVal_Bits [BV{64%N} 0xfff0000000000007%Z]) Mk_annot] Mk_annot) (AExp_Val (AVal_Bits [BV{64%N} 0x0%Z]) Mk_annot) Mk_annot) Mk_annot;
-    Smt (Assert (Binop (Eq) (Manyop (Bvmanyarith Bvand) [Binop ((Bvarith Bvsub)) (Val (Val_Symbolic 29%Z) Mk_annot) (Val (Val_Bits [BV{64%N} 0x8%Z]) Mk_annot) Mk_annot; Val (Val_Bits [BV{64%N} 0xfff0000000000007%Z]) Mk_annot] Mk_annot) (Val (Val_Bits [BV{64%N} 0x0%Z]) Mk_annot) Mk_annot)) Mk_annot;
-    Assume (AExp_Binop (Eq) (AExp_Manyop (Bvmanyarith Bvand) [AExp_Binop ((Bvarith Bvsub)) (AExp_Val (AVal_Var "SP_EL2" []) Mk_annot) (AExp_Val (AVal_Bits [BV{64%N} 0x10%Z]) Mk_annot) Mk_annot; AExp_Val (AVal_Bits [BV{64%N} 0xfff0000000000007%Z]) Mk_annot] Mk_annot) (AExp_Val (AVal_Bits [BV{64%N} 0x0%Z]) Mk_annot) Mk_annot) Mk_annot;
-    Smt (Assert (Binop (Eq) (Manyop (Bvmanyarith Bvand) [Binop ((Bvarith Bvsub)) (Val (Val_Symbolic 29%Z) Mk_annot) (Val (Val_Bits [BV{64%N} 0x10%Z]) Mk_annot) Mk_annot; Val (Val_Bits [BV{64%N} 0xfff0000000000007%Z]) Mk_annot] Mk_annot) (Val (Val_Bits [BV{64%N} 0x0%Z]) Mk_annot) Mk_annot)) Mk_annot;
+    Assume (AExp_Binop (Eq) (AExp_Manyop (Bvmanyarith Bvand) [AExp_Val (AVal_Var "SP_EL2" []) Mk_annot; AExp_Val (AVal_Bits [BV{64%N} 0xfff0000000000007%Z]) Mk_annot] Mk_annot) (AExp_Val (AVal_Bits [BV{64%N} 0x0%Z]) Mk_annot) Mk_annot) Mk_annot;
+    Smt (Assert (Binop (Eq) (Manyop (Bvmanyarith Bvand) [Val (Val_Symbolic 29%Z) Mk_annot; Val (Val_Bits [BV{64%N} 0xfff0000000000007%Z]) Mk_annot] Mk_annot) (Val (Val_Bits [BV{64%N} 0x0%Z]) Mk_annot) Mk_annot)) Mk_annot;
+    Assume (AExp_Binop ((Bvcomp Bvugt)) (AExp_Val (AVal_Var "SP_EL2" []) Mk_annot) (AExp_Val (AVal_Bits [BV{64%N} 0x10%Z]) Mk_annot) Mk_annot) Mk_annot;
+    Smt (Assert (Binop ((Bvcomp Bvugt)) (Val (Val_Symbolic 29%Z) Mk_annot) (Val (Val_Bits [BV{64%N} 0x10%Z]) Mk_annot) Mk_annot)) Mk_annot;
     ReadReg "PSTATE" [Field "SP"] (RegVal_Struct [("SP", RegVal_Base (Val_Bits [BV{1%N} 0x1%Z]))]) Mk_annot;
     ReadReg "PSTATE" [Field "EL"] (RegVal_Struct [("EL", RegVal_Base (Val_Bits [BV{2%N} 0x2%Z]))]) Mk_annot;
     ReadReg "SP_EL2" [] (RegVal_Base (Val_Symbolic 29%Z)) Mk_annot;
