pkvm_handler/wp.v
@@ -3,10 +3,10 @@ Require Import isla.examples.pkvm_handler.instrs.
 
 Definition instrs_iprop `{!islaG Σ} `{!threadG} := ([∗ list] i ∈ instr_map, instr i.1 (Some i.2))%I.
 
-Definition spec_stp `{!islaG Σ} `{!threadG} a sp (v1 v2 : bv 64) : iProp Σ :=
-    ∃ (vold1 vold2 : bv 64),
-    "R0" ↦ᵣ RVal_Bits v1 ∗
-    "R1" ↦ᵣ RVal_Bits v2 ∗
+Definition spec_stp `{!islaG Σ} `{!threadG} a sp : iProp Σ :=
+    ∃ (vold1 vold2 v v': bv 64),
+    "R0" ↦ᵣ RVal_Bits v ∗
+    "R1" ↦ᵣ RVal_Bits v' ∗
     (bv_sub sp [BV{64} 16]) ↦ₘ vold1 ∗
     (bv_sub sp [BV{64} 8]) ↦ₘ vold2 ∗
     ⌜bv_unsigned sp < 2 ^ 52⌝ ∗
@@ -15,17 +15,17 @@ Definition spec_stp `{!islaG Σ} `{!threadG} a sp (v1 v2 : bv 64) : iProp Σ :=
     "SP_EL2" ↦ᵣ RVal_Bits sp ∗
     reg_col sys_regs ∗
     instr_pre a (
-      "R0" ↦ᵣ RVal_Bits v1 ∗
-      "R1" ↦ᵣ RVal_Bits v2 ∗
+      "R0" ↦ᵣ RVal_Bits v ∗
+      "R1" ↦ᵣ RVal_Bits v' ∗
       "SP_EL2" ↦ᵣ RVal_Bits (bv_sub sp [BV{64} 16])∗
       reg_col sys_regs ∗
-      (bv_sub sp [BV{64} 16]) ↦ₘ v1 ∗
-      (bv_sub sp [BV{64} 8]) ↦ₘ v2 ∗
+      (bv_sub sp [BV{64} 16]) ↦ₘ v ∗
+      (bv_sub sp [BV{64} 8]) ↦ₘ v' ∗
       True).
 
-Lemma stp_wp `{!islaG Σ} `{!threadG} (sp v1 v2: bv 64) :
+Lemma stp_wp `{!islaG Σ} `{!threadG} (sp : bv 64) :
   instr 0x7400 (Some a7400) -∗
-  instr_body 0x7400 (spec_stp 0x7404 sp v1 v2).
+  instr_body 0x7400 (spec_stp 0x7404 sp).
 Proof.
   iStartProof.
   unfold spec_stp.
@@ -50,6 +50,8 @@ Definition mrs_regs_64 :=
   (λ r, (KindReg r, BitsShape 64)) <$>
   ["MPAM2_EL2"; "MPAMIDR_EL1"; "MPAM3_EL3"].
 
+Definition mrs_regs :=
+  mrs_regs_32 ++ mrs_regs_64.
 
 Definition exists_reg r :=
   [(KindReg r, BitsShape 64)].
@@ -92,7 +94,6 @@ Definition spec_lsr `{!islaG Σ} `{!threadG} a (v vold : bv 64) : iProp Σ :=
     True
   ).
 
-
 Lemma lsr_wp `{!islaG Σ} `{!threadG} (v vold : bv 64):
   instr 0x7408 (Some a7408) -∗
   instr_body 0x7408 (spec_lsr 0x740c v vold).
@@ -103,4 +104,75 @@ Proof.
   Unshelve.
   all: prepare_sidecond.
   by bits_simplify.
+Qed.
+
+Definition spec `{!islaG Σ} `{!threadG} (sp forward_smc_addr: bv 64) (esr : bv 32) : iProp Σ :=
+  ∃ v0 v1 v5 v6: bv 64,
+  reg_col sys_regs ∗
+  reg_col mrs_regs ∗
+  reg_col CNVZ_regs ∗
+  (* Move to sys_regs *)
+  "InGuardedPage" ↦ᵣ RVal_Bool false ∗
+  "ESR_EL2" ↦ᵣ RVal_Bits esr ∗
+  "R0" ↦ᵣ RVal_Bits v0 ∗
+  "R1" ↦ᵣ RVal_Bits v1 ∗
+  "R5" ↦ᵣ RVal_Bits v5 ∗
+  "R6" ↦ᵣ RVal_Bits v6 ∗
+  "SP_EL2" ↦ᵣ RVal_Bits sp ∗
+  (bv_sub sp [BV{64} 16]) ↦ₘ? 8 ∗
+  (bv_sub sp [BV{64} 8]) ↦ₘ? 8 ∗
+  ⌜bv_unsigned sp < 2 ^ 52⌝ ∗
+  ⌜bv_unsigned sp > 16⌝ ∗
+  ⌜bv_unsigned sp `mod` 8 = 0⌝ ∗
+  [BV{64} 0x77f8] ↦ₘ forward_smc_addr ∗
+  (instr_pre 0x6800 (⌜Z.shiftr (bv_unsigned esr) 26 ≠ 22⌝ ∗ ∃ (v : bv 64), "R0" ↦ᵣ RVal_Bits v ∗ ⌜bv_unsigned v ≠ 22⌝ ∗ True) ∧
+  instr_pre 0x6800 (⌜Z.shiftr (bv_unsigned esr) 26 = 22⌝ ∗ ⌜Z.ge (bv_unsigned v0) 3⌝ ∗ True)) ∗
+  (* Possibly should handle that this address gets shifted (even if it's by zero in this code) *)
+  instr_pre (bv_unsigned forward_smc_addr) (
+    ⌜Z.shiftr (bv_unsigned esr) 26 = 22⌝ ∗
+    ⌜Z.lt (bv_unsigned v0) 3⌝ ∗
+    "SP_EL2" ↦ᵣ RVal_Bits sp ∗
+    "R5" ↦ᵣ RVal_Bits forward_smc_addr ∗
+    "R6" ↦ᵣ RVal_Bits [BV{64} 0] ∗
+    True).
+
+Lemma wp `{!islaG Σ} `{!threadG} sp esr forward_smc_addr:
+  instr 29696 (Some a7400) ∗
+  instr 29700 (Some a7404) ∗
+  instr 29704 (Some a7408) ∗
+  instr 29708 (Some a740c) ∗
+  instr 29712 (Some a7410) ∗
+  instr 29716 (Some a7414) ∗
+  instr 29720 (Some a7418) ∗
+  instr 29724 (Some a741c) ∗
+  instr 29728 (Some a7420) ∗
+  instr 29732 (Some a7424) ∗
+  instr 29736 (Some a7428) ∗
+  instr 29740 (Some a742c) ∗
+  instr 29744 (Some a7430) ∗
+  instr 29748 (Some a7434) ∗
+  instr 29752 (Some a7438) ∗
+  instr 29756 (Some a743c) -∗
+  instr_body 0x7400 (spec sp forward_smc_addr esr).
+Proof.
+  unfold spec.
+  iStartProof.
+  repeat liAStep; liShow.
+  + iDestruct select (_ ∧ _)%I as "[_ ?]".
+    repeat liAStep; liShow.
+  + iDestruct select (_ ∧ _)%I as "[? _]".
+    repeat liAStep; liShow.
+  Unshelve.
+  all: prepare_sidecond.
+  all: try bv_solve.
+  * rewrite <- H4.
+    assert(G: bv_unsigned (bv_concat 64 [BV{32} 0] esr) = bv_unsigned esr); [bv_solve|].
+    by rewrite G in H3.
+  * rewrite <- H4.
+    assert(G: bv_unsigned (bv_concat 64 [BV{32} 0] esr) = bv_unsigned esr); [bv_solve|].
+    by rewrite G in H3.
+  * contradict H4.
+    rewrite H3.
+    rewrite <- H4.
+    by bits_simplify.
 Qed.
