pkvm_handler/a7424_spec.v
@@ -1,0 +1,16 @@
+Require Import isla.isla.
+Require Import isla.aarch64.aarch64.
+Require Export isla.examples.pkvm_handler.a7424.
+
+Lemma a7424_spec `{!islaG Σ} `{!threadG} pc:
+  instr pc (Some a7424) -∗
+  instr_body pc (ldr_mapsto_spec pc 0x7424 "R5" [BV{64} 0x77f8]).
+Proof.
+  iStartProof.
+  repeat liAStep; liShow.
+  Unshelve. all: prepare_sidecond.
+Qed.
+
+Definition a7424_spec_inst `{!islaG Σ} `{!threadG} pc :=
+  entails_to_simplify_hyp 0 (a7424_spec pc).
+Global Existing Instance a7424_spec_inst.
