pkvm_handler/a7430_spec.v
@@ -1,0 +1,17 @@
+Require Import isla.isla.
+Require Import isla.aarch64.aarch64.
+Require Export isla.examples.pkvm_handler.a7430.
+
+Lemma a7430_spec `{!islaG Σ} `{!threadG} pc:
+  instr pc (Some a7430) -∗
+  instr_body pc (movk_spec pc "R6" 0 0).
+Proof.
+  iStartProof.
+  repeat liAStep; liShow.
+  Unshelve. all: prepare_sidecond.
+  by bits_simplify.
+Qed.
+
+Definition a7430_spec_inst `{!islaG Σ} `{!threadG} pc :=
+  entails_to_simplify_hyp 0 (a7430_spec pc).
+Global Existing Instance a7430_spec_inst.
